\chapter{Brownian Motion}

\begin{definition}[Brownian Motion (1)]
	A real-valued stochastic process \(B(t),t\geq 0\) is said to be Brownian motion, if
	\begin{enumerate}
		\item for any \(0=t_{0}\leq t_{1}\leq\cdots\leq t_{n}\) the increments
		      \begin{equation*}
			      B\left(t_{1}\right)-B\left(t_{0}\right),\ldots,B\left(t_{n}\right)-B\left(t_{n-1}\right)
		      \end{equation*}
		      are independent
		\item for any \(s,t\geq 0\) and Borel sets \(A\in\bbR\),
		      \begin{equation}
			      P\left(B(s+t)-B(s)\in A\right)=\int_{A}(2\pi t)^{-1/2}\exp\left(-x^{2}/2t\right)\dif x
		      \end{equation}
		\item the sample paths \(t\rightarrow B(t)\) are a.s.\ continuous.
	\end{enumerate}
\end{definition}

\begin{property}
	For a one-dimensional Brownian motion, if \(B(0)=0\), then we have the following properties
	\begin{enumerate}
		\item \(EB_{t}=0,\Var\left(B_{t}\right)=t,\quad t\geq 0\).
		\item \(\operatorname{Cov}\left(B_{s},B_{t}\right)=s,\operatorname{Corr}\left(B_{s},B_{t}\right)=\sqrt{\frac{s}{t}},\quad\forall 0\leq s\leq t\).
	\end{enumerate}
\end{property}

\begin{proof}
	\begin{enumerate}
		\item Since \(B_{t}=B_{t}-B_{0}\sim N(0, t)\), then we have
		      \begin{equation*}
			      EB_{t}=0,\Var\left(B_{t}\right)=t
		      \end{equation*}
		\item Suppose \(0\leq s\leq t\),
		      \begin{equation*}
			      \operatorname{Cov}\left(B_{s}, B_{t}\right)=E\left[\left(B_{s}-EB_{s}\right)\left(B_{t}-EB_{t}\right)\right]=EB_{s}B_{t}
		      \end{equation*}
		      Let \(B_{t}=\left(B_{t}-B_{s}\right)+B_{s}\), we have
		      \begin{equation*}
			      \begin{aligned}
				      EB_{s}B_{t} & =E\left[B_{s}\cdot\left(\left(B_{t}-B_{s}\right)+B_{s}\right)\right] \\
				                  & =E\left[B_{s}\cdot\left(B_{t}-B_{s}\right)\right]+EB_{s}^{2}
			      \end{aligned}
		      \end{equation*}
		      Since \(B_{s}=B_{s}-B_{0}\) and \(B_{t}-B_{s}\) are independent,
		      \begin{equation*}
			      E\left[B_{s} \cdot\left(B_{t}-B_{s}\right)\right]=EB_{s} \cdot E\left[B_{t}-B_{s}\right]=0
		      \end{equation*}
		      Thus
		      \begin{equation*}
			      \operatorname{Cov}\left(B_{s}, B_{t}\right)=EB_{s}^{2}=s
		      \end{equation*}
		      And
		      \begin{equation*}
			      \operatorname{Corr}\left(B_{s},B_{t}\right)=\frac{\operatorname{Cov}\left(B_{s},B_{t}\right)}{\sigma_{B_{s}}\sigma_{B_{t}}}=\frac{s}{\sqrt{st}}=\sqrt{\frac{s}{t}}
		      \end{equation*}
	\end{enumerate}
\end{proof}

A second equivalent definition of Brownian motion is as follows,

\begin{definition}[Brownian Motion (2)]
	A real-valued stochastic process \(B(t),t\geq 0\), \textbf{starting from \(0\)}, is said to be Brownian motion, if
	\begin{enumerate}
		\item \(B(t)\) is a Gaussian process\footnote{Gaussian process, i.e., all its finite-dimensional distributions are multivariate normal.}
		\item \(\forall s,t\geq 0,EB_{s}=0\) and \(EB_{s}B_{t}=s\wedge t\)
		\item the sample paths \(t\rightarrow B(t)\) are a.s.\ continuous
	\end{enumerate}
\end{definition}

\section{Markov Properties}

\section{Martingales}

\begin{example}[Quadratic Martingale]
	Suppose \(B_{t}\) is a Brownian motion, then \(B_{t}^{2}-t\) is a martingale.
\end{example}

\begin{proof}
	Let \(B_{t}^{2}=\left(B_{s}+B_{t}-B_{s}\right)^{2}\), we have
	\begin{equation*}
		\begin{aligned}
			E_{x}\left(B_{t}^{2}\mid\mcF_{s}\right) & =E_{x}\left(B_{s}^{2}+2 B_{s}\left(B_{t}-B_{s}\right)+\left(B_{t}-B_{s}\right)^{2} \mid \mcF_{s}\right)                     \\
			                                        & =B_{s}^{2}+2 B_{s} E_{x}\left(B_{t}-B_{s} \mid \mcF_{s}\right)+E_{x}\left(\left(B_{t}-B_{s}\right)^{2} \mid \mcF_{s}\right) \\
			                                        & =B_{s}^{2}+0+(t-s)
		\end{aligned}
	\end{equation*}
	since \(B_{t}-B_{s}\) is independent of \(\mcF_{s}\) and has mean 0 and variance \(t-s\).
\end{proof}

\begin{example}[Exponential Martingale]
	Suppose \(B_{t}\) is a Brownian motion, then \(\exp\left(\theta B_{t}-\left(\theta^{2}t/2\right)\right)\) is a martingale.
\end{example}

\begin{proof}
	Let \(B_{t}=B_{t}-B_{s}+B_{s}\), then
	\begin{equation*}
		\begin{aligned}
			E_{x}\left(\exp\left(\theta B_{t}\right)\mid\mcF_{s}\right) & =\exp \left(\theta B_{s}\right)E\left(\exp\left(\theta\left(B_{t}-B_{s}\right)\right)\mid\mcF_{s}\right) \\
			                                                            & =\exp\left(\theta B_{s}\right)\exp\left(\theta^{2}(t-s)/2\right)
		\end{aligned}
	\end{equation*}
	since \(B_{t}-B_{s}\) is independent of \(\mcF_{s}\) and has mean 0 and variance \(t-s\). Thus
	\begin{equation*}
		\begin{aligned}
			E_{x}\left(\exp\left(\theta B_{t}-\left(\theta^{2}t/2\right)\right)\mid\mcF_{s}\right) & =E_{x}\left(\exp\left(\theta B_{t}\right)\mid\mcF_{s}\right)\cdot\exp\left(-\left(\theta^{2}t/2\right)\right) \\
			                                                                                       & =\exp\left(\theta B_{s}-\left(\theta^{2}s/2\right)\right)
		\end{aligned}
	\end{equation*}
\end{proof}

\begin{theorem}[LÃ©vy's Martingale Characterization]
	Let \(B(t),t\geq 0\), be a real-valued stochastic process and let \(\mcF_{t}=\sigma\left(B_{s},s\leq t\right)\) be the filtration generated by it. Then \(B(t)\) is a Brownian motion if and only if
	\begin{enumerate}
		\item \(B(0)=0\) a.s.
		\item the sample paths \(t\rightarrow B(t)\) are continuous a.s.
		\item \(B(t)\) is a martingale with respect to \(\mcF_{t}\)
		\item \(|B(t)|^{2}-t\) is a martingale with respect to \(\mcF_{t}\)
	\end{enumerate}
\end{theorem}

\section{Sample Paths}

Let \(0=t_{0}^{n}<t_{1}^{n}<\cdots<t_{n}^{n}=T\), where \(t_{i}^{n}=\frac{iT}{n}\) be a partition of the interval \([0,T]\) into \(n\) equal parts, and
\begin{equation}
	\Delta_{i}^{n}B=B\left(t_{i+1}^{n}\right)-B\left(t_{i}^{n}\right)
\end{equation}
be the corresponding increments of the Brownian motion \(B(t)\).

\begin{theorem}\label{thm:limited-square-variation}
	\begin{equation}
		\lim_{n\rightarrow\infty}\sum_{i=0}^{n-1}\left(\Delta_{i}^{n}B\right)^{2}=T\quad\text {in}\quad L^{2}
	\end{equation}
\end{theorem}

\begin{proof}
	Since the increments \(\Delta_{i}^{n}B\) are independent and
	\begin{equation*}
		E\left(\Delta_{i}^{n}B\right)=0,\quad E\left(\left(\Delta_{i}^{n}B\right)^{2}\right)=\frac{T}{n},\quad E\left(\left(\Delta_{i}^{n}B\right)^{4}\right)=\frac{3T^{2}}{n^{2}}
	\end{equation*}
	it follows that
	\begin{equation*}
		\begin{aligned}
			E\left(\left[\sum_{i=0}^{n-1}\left(\Delta_{i}^{n}B\right)^{2}-T\right]^{2}\right)= & E\left(\left[\sum_{i=0}^{n-1}\left(\left(\Delta_{i}^{n}B\right)^{2}-\frac{T}{n}\right)\right]^{2}\right)                                                   \\
			=                                                                                  & \sum_{i=0}^{n-1}E\left[\left(\left(\Delta_{i}^{n}B\right)^{2}-\frac{T}{n}\right)^{2}\right]                                                                \\
			=                                                                                  & \sum_{i=0}^{n-1}\left[E\left(\left(\Delta_{i}^{n}B\right)^{4}\right)-\frac{2T}{n}E\left(\left(\Delta_{i}^{n}B\right)^{2}\right)+\frac{T^{2}}{n^{2}}\right] \\
			=                                                                                  & \sum_{i=0}^{n-1}\left[\frac{3T^{2}}{n^{2}}-\frac{2T^{2}}{n^{2}}+\frac{T^{2}}{n^{2}}\right]                                                                 \\
			=                                                                                  & \frac{2T^{2}}{n}\rightarrow 0,\quad n\rightarrow\infty
		\end{aligned}
	\end{equation*}
\end{proof}

\begin{definition}[Variation]
	The variation of a function \(f:[0,T]\rightarrow\bbR\) is defined to be
	\begin{equation}
		\limsup_{\Delta t\rightarrow 0}\sum_{i=0}^{n-1}\left|f\left(t_{i+1}\right)-f\left(t_{i}\right)\right|
	\end{equation}
	where \(t=\left(t_{0},t_{1},\ldots,t_{n}\right)\) is a partition of \([0,T]\), i.e. \(0=t_{0}<t_{1}<\cdots<t_{n}=T\), and where
	\begin{equation}
		\Delta t=\max_{i=0,\ldots,n-1}\left|t_{i+1}-t_{i}\right|
	\end{equation}
\end{definition}

\begin{theorem}
	The variation of the paths of \(B(t)\) is infinite a.s..
\end{theorem}

\begin{proof}
	Consider the sequence of partitions \(t^{n}=\left(t_{0}^{n},t_{1}^{n},\ldots,t_{n}^{n}\right)\) of \([0,T]\) into \(n\) equal parts. Then
	\begin{equation*}
		\sum_{i=0}^{n-1}\left|\Delta_{i}^{n}B\right|^{2}\leq\left(\max_{i=0,\ldots,n-1}\left|\Delta_{i}^{n}B\right|\right)\sum_{i=0}^{n-1}\left|\Delta_{i}^{n}B\right|
	\end{equation*}

	Since the paths of \(B(t)\) are a.s.\ continuous on \([0,T]\),
	\begin{equation*}
		\lim_{n\rightarrow\infty}\left(\max_{i=0,\ldots,n-1}\left|\Delta_{i}^{n}B\right|\right)=0\quad\text{a.s. }
	\end{equation*}

	By Theorem~\ref{thm:limited-square-variation}, we have
	\begin{equation*}
		\lim_{n\rightarrow\infty}\sum_{i=0}^{n-1}\left(\Delta_{i}^{n}B\right)^{2}=T\ \text{in}\ L^{2}
	\end{equation*}
	Since every sequence of random variables convergent in \(L^{2}\) has a subsequence convergent a.s. There is a subsequence \(t^{n_{k}}=\left(t_{0}^{n_{k}},t_{1}^{n_{k}},\ldots,t_{n_{k}}^{n_{k}}\right)\) of partitions such that
	\begin{equation*}
		\lim_{k\rightarrow\infty}\sum_{i=0}^{n_{k}-1}\left|\Delta_{i}^{n_{k}}B\right|^{2}=T\quad\text{a.s. }
	\end{equation*}

	Since
	\begin{equation*}
		\sum_{i=0}^{n_{k}-1}\left|\Delta_{i}^{n_{k}}B\right|\geq\frac{\sum_{i=0}^{n_{k}-1}\left|\Delta_{i}^{n_{k}}B\right|^{2}}{\max_{i=0,\ldots,n_{k}-1}\left|\Delta_{i}^{n_{k}}B\right|}
	\end{equation*}
	hence,
	\begin{equation*}
		\lim_{k\rightarrow\infty}\sum_{i=0}^{n_{k}-1}\left|\Delta_{i}^{n_{k}}B\right|=\infty\quad\text{a.s. }
	\end{equation*}
	while
	\begin{equation*}
		\lim_{k\rightarrow\infty}\Delta t^{n_{k}}=\lim_{k\rightarrow\infty}\frac{T}{n_{k}}=0
	\end{equation*}
\end{proof}

\section{It\^o Stochastic Calculus}

\begin{definition}[It\^o Stochastic Integral]
	For any \(T>0\) we shall denote by \(M_{T}^{2}\) the space of all stochastic processes \(f(t), t \geq 0\) such that
	\begin{equation*}
		1_{[0,T)}f\in M^{2}
	\end{equation*}
	The It\^o stochastic integral (from \(0\) to \(T\)) of \(f\in M_{T}^{2}\) is defined by
	\begin{equation}
		I_{T}(f)=I\left(1_{[0,T)}f\right)
	\end{equation}
	which can be denoted by
	\begin{equation}
		\int_{0}^{T}f(t)\dif B(t)
	\end{equation}
\end{definition}

\begin{property}
	The It\^o Stochastic Integral has the following properties:
	\begin{enumerate}
		\item Linearity: For \(\forall f,g\in M_{t}^{2}\), \(\forall \alpha,\beta\in\bbR\),
		      \begin{equation}
			      \int_{0}^{t}(\alpha f(r)+\beta g(r))\dif B(r)=\alpha \int_{0}^{t}f(r)\dif B(r)+\beta\int_{0}^{t}g(r)\dif B(r)
		      \end{equation}
		\item Isometry: For \(\forall f\in M_{t}^{2}\),
		      \begin{equation}
			      E\left(\left|\int_{0}^{t}f(r)\dif B(r)\right|^{2}\right)=E\left(\int_{0}^{t}|f(r)|^{2}\dif r\right)
		      \end{equation}
		\item Martingale Property: For \(\forall f\in M_{t}^{2}\) and  \(\forall 0\leq s<t\),
		      \begin{equation}
			      E\left(\int_{0}^{t}f(r)\dif B(r)\mid\mcF_{s}\right)=\int_{0}^{s}f(r)\dif B(r)
		      \end{equation}
	\end{enumerate}
\end{property}

\begin{proof}

\end{proof}

\begin{definition}[It\^o Process]
	A stochastic process \(\xi(t),t\geq 0\) is said to be an It\^o process if it has a.s.\ continuous paths and can be represented as
	\begin{equation}
		\xi(T)=\xi(0)+\int_{0}^{T}a(t)\dif t+\int_{0}^{T}b(t)\dif B(t)\quad\text{a.s.}
	\end{equation}
	where \(b(t)\) is a process belonging to \(M_{T}^{2}\) for all \(T>0\) and \(a(t)\) is a process adapted to the filtration \(\mcF_{t}\) such that
	\begin{equation}
		\int_{0}^{T}|a(t)|\dif t<\infty\quad\text {a.s.} \label{eq:condition-of-process-adapted-to-filtration}
	\end{equation}
	for all \(T\geq 0\).
	The It\^o process is denoted by
	\begin{equation}
		\dif\xi(t)=a(t)\dif t+b(t)\dif B(t)
	\end{equation}
\end{definition}

\begin{remark}
	The class of all adapted processes \(a(t)\) satisfying~\ref{eq:condition-of-process-adapted-to-filtration} for some \(T>0\) will be denoted by \(\mathcal{L}_{T}^{1}\).
\end{remark}

\begin{theorem}[It\^o Formula]
	Suppose \(F\left(t,x\right)\) is a real-valued function with continuous partial derivatives \(F_{t}^{\prime}\left(t,x\right)\), \(F_{x}^{\prime}\left(t,x\right)\) and \(F_{xx}^{\prime\prime}\left(t,x\right)\) for all \(t\geq 0\) and \(x\in\bbR\).
	\begin{enumerate}
		\item If \(\xi(t)\) be an It\^o process
		      \begin{equation*}
			      \xi(t)=\xi(0)+\int_{0}^{t}a(s)\dif s+\int_{0}^{t}b(s)\dif B(s)
		      \end{equation*}
		      and the process \(b(t)F_{x}^{\prime}(t,\xi(t))\) belongs to \(M_{T}^{2}\) for all \(T\geq 0\). Then \(F(t,\xi(t))\) is an It\^o process such that
		      \begin{equation}
			      \begin{aligned}
				      \dif F(t,\xi(t))= & \left(F_{t}^{\prime}(t,\xi(t))+F_{x}^{\prime}(t,\xi(t))a(t)+\frac{1}{2}F_{xx}^{\prime\prime}(t,\xi(t))b(t)^{2}\right)\dif t \\
				                        & +F_{x}^{\prime}(t,\xi(t))b(t)\dif B(t)
			      \end{aligned}
		      \end{equation}
		\item If \(\xi(t)\) be an Brownian Motion, such that \(\xi(t)=B(t)\), and the process \(F_{x}^{\prime}(t,B(t))\) belongs to \(M_{T}^{2}\) for all \(T \geq 0\). Then \(F(t,B(t))\) is an It\^o process such that
		      \begin{equation}
			      \dif F(t,B(t))=\left(F_{t}^{\prime}(t,B(t))+\frac{1}{2}F_{xx}^{\prime\prime}(t,B(t))\right)\dif t+F_{x}^{\prime}(t,B(t))\dif B(t)
		      \end{equation}
	\end{enumerate}
\end{theorem}

\begin{example}[Exponential Martingale]
	Show that the exponential martingale
	\begin{equation*}
		X(t)=\mathrm{e}^{B(t)}\mathrm{e}^{-\frac{t}{2}}
	\end{equation*}
	is an It\^o process, and satisfies the equation
	\begin{equation*}
		\dif X(t)=X(t)\dif B(t)
	\end{equation*}
\end{example}
\begin{proof}
	Let \(F(t,x)=\mathrm{e}^{x}\mathrm{e}^{-\frac{t}{2}}\), then we have
	\begin{equation*}
		F_{t}^{\prime}(t,x)=-\frac{1}{2}F(t,x),\quad F_{x}^{\prime}(t,x)=F(t,x),\quad F_{xx}^{\prime\prime}(t,x)=F(t,x)
	\end{equation*}
	thus, by It\^o Formula, we have
	\begin{equation*}
		\begin{aligned}
			\dif X(t)= & \dif F(t,B(t))=\left(F_{t}^{\prime}(t,B(t))+\frac{1}{2}F_{xx}^{\prime\prime}(t,B(t))\right)\dif t+F_{x}^{\prime}(t,B(t))\dif B(t) \\
			=          & \left(-\frac{1}{2}F(t,B(t))+\frac{1}{2}F(t,B(t))\right)\dif t+F(t,B(t))\dif B(t)                                                  \\
			=          & X(t)\dif B(t)
		\end{aligned}
	\end{equation*}
\end{proof}

\begin{example}

\end{example}

\begin{example}

\end{example}
