\chapter{Support Vector Machine}

\begin{theorem}
	The minimizer of
	\begin{equation*}
		f^{*}(X)=\arg\min_{f}\bbE\left\{\left[1-f(X)Y\right]_{+}\mid X=x\right\}
	\end{equation*}
	is the sign of \(f(x)=\log\frac{p(x)}{1-p(x)}\), i.e., \(\text{sgn}\left[p(x)-\frac{1}{2}\right]\).
\end{theorem}

\begin{proof}
	Consider the hinge loss function:
	\begin{equation*}
		\begin{aligned}
			  & \bbE\left\{\left[1 - Yg(X)\right]_{+} \mid X = x\right\}                                                             \\
			= & \left[1 - g(x)\right]_{+} P\left(Y = 1 \mid X = x\right) + \left[1 + g(x)\right]_{+} P\left(Y = -1 \mid X = x\right) \\
			= & \left[1 - g(x)\right]_{+} p(x) + \left[1 + g(x)\right]_{+} \left[1 - p(x)\right]                                     \\
			= & \begin{cases}
				    \left[1 - g(x)\right] p(x),                  & g(x) < -1           \\
				    1 + \left[1 - 2p(x)\right] g(x),             & -1 \leq g(x) \leq 1 \\
				    \left[1 + g(x)\right] \left[1 - p(x)\right], & g(x) > 1
			    \end{cases}
		\end{aligned}
	\end{equation*}

	For \(g(x) < -1\):
	\begin{equation*}
		\arg\min_{g} \bbE\left\{\left[1 - Yg(X)\right]_{+} \mid X = x\right\} = \arg\min_{g} \left[1 - g(x)\right] p(x) = -1
	\end{equation*}

	For \(g(x) > 1\):
	\begin{equation*}
		\arg\min_{g} \bbE\left\{\left[1 - Yg(X)\right]_{+} \mid X = x\right\} = \arg\min_{g} \left[1 + g(x)\right] \left[1 - p(x)\right] = 1
	\end{equation*}

	For \(-1 \leq g(x) \leq 1\):
	\begin{equation*}
		\begin{aligned}
			  & \arg\min_{g} \bbE\left\{\left[1 - Yg(X)\right]_{+} \mid X = x\right\} \\
			= & \arg\min_{g} \left\{1 + \left[1 - 2p(x)\right] g(x)\right\}           \\
			= & \begin{cases}
				    -1, & p(x) < \frac{1}{2} \\
				    0,  & p(x) = \frac{1}{2} \\
				    1,  & p(x) > \frac{1}{2}
			    \end{cases}
		\end{aligned}
	\end{equation*}

	Therefore, the minimizer \(g^*(x)\) of \(\bbE\left\{\left[1 - Yg(X)\right]_{+} \mid X = x\right\}\) is the sign of \(p(x) - \frac{1}{2}\), which is also the sign of \(f(x) = \log \frac{p(x)}{1 - p(x)}\).
\end{proof}
