\chapter{Binary Data}

\section{Model Assumption}

Suppose
\begin{equation}
    Y\sim b\left(m,\pi\right),\quad i=1,2,\ldots,n
\end{equation}
with link function
\begin{equation}
    \eta=g\left(\pi\right)=\log\left(\frac{\pi}{1-\pi}\right)=\mathbf{x}^{\prime}\boldsymbol{\beta}
\end{equation}
\begin{remark}
    
\end{remark}

\section{Model Estimation}

The likelihood function is
\begin{equation}
    f\left(\boldsymbol{\pi}\mid\mathbf{X},\mathbf{y}\right)=\prod_{i=1}^{n}\binom{m_{i}}{y_{i}}\pi_{i}^{y_{i}}\left(1-\pi_{i}\right)^{m_{i}-y_{i}}
\end{equation}
and the log-likelihood function is
\begin{equation}
    \begin{aligned}
        \ell\left(\boldsymbol{\beta}\right)= & \log\left[f\left(\boldsymbol{\pi}\mid\mathbf{X},\mathbf{y}\right)\right]=\sum_{i=1}^{n}\ell_{i}\left(\boldsymbol{\beta}\right)                                 \\
        =                                    & \sum_{i=1}^{n}\left\{\log\left[\binom{m_{i}}{y_{i}}\right]+y_{i}\log\left(\pi_{i}\right)+\left(m_{i}-y_{i}\right)\log\left(1-\pi_{i}\right)\right\}            \\
        =                                    & \sum_{i=1}^{n}\left[y_{i}\log\left(\frac{\pi_{i}}{1-\pi_{i}}\right)+m_{i}\log\left(1-\pi_{i}\right)\right]+\sum_{i=1}^{n}\log\left[\binom{m_{i}}{y_{i}}\right]
    \end{aligned}
\end{equation}
where
\begin{equation}
    \pi_{i}=\frac{\exp\left(\mathbf{x}_{i}^{\prime}\boldsymbol{\beta}\right)}{1+\exp\left(\mathbf{x}_{i}^{\prime}\boldsymbol{\beta}\right)}
\end{equation}

Thus,
\begin{gather*}
    U_{r}\left(\boldsymbol{\beta}\right)=\sum_{i=1}^{n}\left(y_{i}-m_{i}\pi_{i}\right)x_{ir} \\
    I_{sr}\left(\boldsymbol{\beta}\right)=\sum_{i=1}^{n}m_{i}\pi_{i}\left(1-\pi_{i}\right)x_{is}x_{ir}
\end{gather*}