\chapter{Central Limit Theorems}

\begin{introduction}
    \item The De Moivre-Laplace Theorem
    \item Central Limit Theorem for i.i.d Sequences
    \item The Linderberg-Feller Central Limit Theorem
\end{introduction}

\section{The De Moivre-Laplace Theorem}

\begin{lemma}{Stirling's Formula}{stirling}
    \begin{equation}
        n ! \sim \sqrt{2 \pi} n^{n+\frac{1}{2}} e^{-n} \text{ as } n \rightarrow \infty.
    \end{equation}
\end{lemma}

\begin{proof}

\end{proof}

\begin{lemma}{}{exp}
    If $c_j\rightarrow 0$, $a_j\rightarrow\infty$ and $a_jc_j\rightarrow\lambda$, then
    \begin{equation}
        \left(1+c_j\right)^{a_j}\rightarrow e^\lambda.
    \end{equation}
\end{lemma}

\begin{proof}

\end{proof}

\begin{theorem}{The De Moivre-Laplace Theorem}{de-moivre-laplace}
    Let $X_{1}, X_{2}, \ldots$ be i.i.d. with $P\left(X_{1}=1\right)=P\left(X_{1}=-1\right)=1 / 2$ and let $S_{n}=X_{1}+\cdots+X_{n}$. If $a<b$, then as $m \rightarrow \infty$
    \begin{equation}
        P\left(a \leq S_{m} / \sqrt{m} \leq b\right) \rightarrow \int_{a}^{b}(2 \pi)^{-1 / 2} e^{-x^{2} / 2} \mathrm{d} x.
    \end{equation}
\end{theorem}

\begin{proof}
    If $n$ and $k$ and integers
    \begin{equation*}
        P\left(S_{2 n}=2 k\right)=\left(\begin{array}{c}
                2 n \\
                n+k
            \end{array}\right) 2^{-2 n}
    \end{equation*}
    By lemma \ref{lem:stirling}, we have
    \begin{equation*}
        \begin{aligned}
            \left(\begin{array}{c}
                    2 n \\
                    n+k
                \end{array}\right) & =\frac{(2 n) !}{(n+k) !(n-k) !}                                                                                             \\
                                                   & \sim \frac{(2 n)^{2 n}}{(n+k)^{n+k}(n-k)^{n-k}} \cdot \frac{(2 \pi(2 n))^{1 / 2}}{(2 \pi(n+k))^{1 / 2}(2 \pi(n-k))^{1 / 2}}
        \end{aligned}
    \end{equation*}
    Hence,
    \begin{equation*}
        \begin{aligned}
            P\left(S_{2 n}=2 k\right) & =
            \left(\begin{array}{c}
                    2 n \\
                    n+k
                \end{array}\right) 2^{-2 n}                                                                                               \\
                                      & \sim\left(1+\frac{k}{n}\right)^{-n-k} \cdot\left(1-\frac{k}{n}\right)^{-n+k}                                      \\
                                      & \cdot(\pi n)^{-1 / 2} \cdot\left(1+\frac{k}{n}\right)^{-1 / 2} \cdot\left(1-\frac{k}{n}\right)^{-1 / 2}           \\
                                      & =\left(1-\frac{k^{2}}{n^{2}}\right)^{-n} \cdot\left(1+\frac{k}{n}\right)^{-k} \cdot\left(1-\frac{k}{n}\right)^{k} \\
                                      & \cdot(\pi n)^{-1 / 2} \cdot\left(1+\frac{k}{n}\right)^{-1 / 2} \cdot\left(1-\frac{k}{n}\right)^{-1 / 2}           \\
        \end{aligned}
    \end{equation*}
    Let $2k=x\sqrt{2n}$, i.e., $k=x\sqrt{\frac{n}{2}}$. By lemma \ref{lem:exp}, we have
    \begin{equation*}
        \begin{aligned}
            \left(1-\frac{k^{2}}{n^{2}}\right)^{-n} & =\left(1-x^{2} / 2 n\right)^{-n} \rightarrow e^{x^{2} / 2}       \\
            \left(1+\frac{k}{n}\right)^{-k}         & =(1+x / \sqrt{2 n})^{-x \sqrt{n / 2}} \rightarrow e^{-x^{2} / 2} \\
            \left(1-\frac{k}{n}\right)^{k}          & =(1-x / \sqrt{2 n})^{x \sqrt{n / 2}} \rightarrow e^{-x^{2} / 2}
        \end{aligned}
    \end{equation*}
    For this choice of $k$, $k/n \rightarrow 0$, so
    \begin{equation*}
        \left(1+\frac{k}{n}\right)^{-1 / 2} \cdot\left(1-\frac{k}{n}\right)^{-1 / 2} \rightarrow 1.
    \end{equation*}
    Putting things together, we have
    \begin{equation*}
        P\left(S_{2 n}=2 k\right) \sim (\pi n)^{-1 / 2} e^{-x^{2} / 2}, \text{ as } \frac{2k}{\sqrt{2n}} \rightarrow x.
    \end{equation*}
    Therefore,
    \begin{equation*}
        P\left( a\sqrt{2n} \leq S_{2 n} \leq b\sqrt{2 n} \right) = \sum_{m \in \left[a\sqrt{2 n},b\sqrt{2 n}\right] \cap 2\mathbb{Z}} P\left(S_{2 n}=m\right)
    \end{equation*}
    Let $m=x\sqrt{2 n}$, we have that this is
    \begin{equation*}
        \approx \sum_{x \in \left[a,b\right] \cap \left(2\mathbb{Z} / \sqrt{2 n}\right)}(2 \pi)^{-1 / 2} e^{-x^{2} / 2}\cdot(2/n)^{1/2}
    \end{equation*}
    where $2\mathbb{Z} / \sqrt{2 n} = \left\{2z/\sqrt{2n} : z\in\mathbb{Z}\right\}$. As $n\rightarrow\infty$, the sum just shown is
    \begin{equation*}
        \approx \int_{a}^{b}(2 \pi)^{-1 / 2} e^{-x^{2} / 2} \mathrm{d} x.
    \end{equation*}
    To remove the restriction to even integers, observe $S_{2 n +1}=S_{2 n} \pm 1$.\\
    Let $m=2n$, as $m\rightarrow\infty$,
    \begin{equation*}
        P\left(a \leq S_{m} / \sqrt{m} \leq b\right) \rightarrow \int_{a}^{b}(2 \pi)^{-1 / 2} e^{-x^{2} / 2} \mathrm{d} x.
    \end{equation*}
\end{proof}

\section{Central Limit Theorems}

\begin{theorem}{Central Limit Theorem for i.i.d. Sequences}{}
    Let $X_1,X_2,\ldots$ be i.i.d. with $EX_i=\mu$, $\text{Var}(X_i)=\sigma^2\in(0,\infty)$. Let $S_n=X_1+X_2+\ldots+X_n$, then
    \begin{equation}
        \frac{S_n-n\mu}{\sigma n^{\frac{1}{2}}} \stackrel{d}{\rightarrow} \chi,
    \end{equation}
    where $\chi$ has the standard normal distribution.
\end{theorem}

\begin{proof}

\end{proof}

\begin{theorem}{The Linderberg-Feller Central Limit Theorem}{}
    For each $n$, let $X_{n,m},1\leq m\leq n$, be independent random variables with $EX_{n,m}=0$. If
    \begin{enumerate}
        \item $\sum_{m=1}^{n}EX_{n,m}^{2} \rightarrow \sigma^{2}>0$.
        \item $\forall\epsilon>0,\lim_{n\rightarrow\infty}\sum_{m=1}^{n}E\left(\left|X_{n,m}\right|^{2};\left|X_{n,m}\right|>\epsilon\right)=0$
    \end{enumerate}
    Then $S_{n}=X_{n,1}+\cdots+X_{n,n}\stackrel{d}{\rightarrow}\sigma\chi$ as $n\rightarrow\infty$.
\end{theorem}

\begin{proof}

\end{proof}
